Use auxilliary trivial mutual inductive to prove well-foundedness

src/named/Pf.v
@@ -6,7 +6,7 @@ Set Bullet Behavior "Strict Subproofs".
 
 Require Import String.
 From Utils Require Import Utils.
-Require Import Named.Exp Named.ARule.
+From Named Require Import Exp ARule Matches ImCore.
 Import OptionMonad.
 
 (* Proofs of relatedness; todo: separate sort from term pf? *)
@@ -109,9 +109,24 @@ Fixpoint get_subseq {A} (args : list string) (l : named_list A) :=
     else get_subseq args l'
   | _::_,[::]=> None
   end.
+
+                 
+Lemma get_subseq_exact (s : subst)
+  : Some s = get_subseq (map fst s) s.
+Proof.
+  induction s; intros; break; simpl in *; auto.
+  rewrite ?eq_refl.
+  rewrite <-IHs; eauto.
+Qed.
+
+Lemma get_subseq_nil (s : subst)
+  : Some [::] = get_subseq [::] s.
+Proof.
+  destruct s; simpl; reflexivity.
+Qed.
              
 Section RuleChecking.
-  Context (l : lang).
+  Context (l : lang) (wfl : wf_lang l).
 
   Section InnerLoop.
     Context (synth_le_term : pf -> ctx -> option (sort*exp*exp)).
@@ -237,15 +252,360 @@ Section RuleChecking.
          ret (t1,e1,e2)
   end.
 
+  Inductive pf_term_ind : pf -> Set :=
+  | ind_var x : pf_term_ind (pvar x)
+  | ind_con n pl : pf_args_ind pl -> pf_term_ind (pcon n pl)
+  | ind_ax n pl : pf_args_ind pl -> pf_term_ind (ax n pl)
+  | ind_sym p : pf_term_ind p -> pf_term_ind (sym p)
+  | ind_trans p1 p2 : pf_term_ind p1 -> pf_term_ind p2 -> pf_term_ind (trans p1 p2)
+  | ind_conv pt p : pf_sort_ind pt -> pf_term_ind p -> pf_term_ind (conv pt p)
+  with pf_args_ind : list pf -> Set :=
+  | pf_args_ind_nil : pf_args_ind [::]
+  | pf_args_ind_cons p pl : pf_args_ind pl -> pf_term_ind p -> pf_args_ind (p::pl)
+  with pf_sort_ind : pf -> Set :=
+    (*TODO: include or no?*)
+  | sind_var x : pf_sort_ind (pvar x)
+  | sind_con n pl : pf_args_ind pl -> pf_sort_ind (pcon n pl)
+  | sind_ax n pl : pf_args_ind pl -> pf_sort_ind (ax n pl)
+  | sind_sym p : pf_sort_ind p -> pf_sort_ind (sym p)
+  | sind_trans p1 p2 : pf_sort_ind p1 -> pf_sort_ind p2 -> pf_sort_ind (trans p1 p2)
+  (* TODO: include or no?*)
+  | sind_conv pt p : pf_sort_ind (conv pt p).
 
-End RuleChecking.
+
+  Section InnerLoop.
+    Context (pf_term_ind_trivial : forall p, pf_term_ind p).
+    Fixpoint pf_args_ind_trivial pl : pf_args_ind pl :=
+          match pl as pl return pf_args_ind pl with
+          | [::] => pf_args_ind_nil
+          | p :: pl' =>
+            pf_args_ind_cons (pf_args_ind_trivial pl') (pf_term_ind_trivial p)
+          end.
+  End InnerLoop.
+
+  Fixpoint pf_term_ind_trivial p : pf_term_ind p :=
+    match p with
+    | pvar x => ind_var x
+    | pcon name pl =>
+      ind_con name (pf_args_ind_trivial pf_term_ind_trivial pl)
+    | ax name pl => ind_ax name (pf_args_ind_trivial pf_term_ind_trivial pl)
+    | sym p' => ind_sym (pf_term_ind_trivial p')
+    | trans p1 p2 =>
+      ind_trans (pf_term_ind_trivial p1) (pf_term_ind_trivial p2)
+    | conv pt p' =>
+      ind_conv (pf_sort_ind_trivial pt) (pf_term_ind_trivial p')
+    end
+  with pf_sort_ind_trivial p : pf_sort_ind p :=
+    match p with
+    | pvar x => sind_var x
+    | pcon name pl => sind_con name (pf_args_ind_trivial pf_term_ind_trivial pl)
+    | ax name pl => sind_ax name (pf_args_ind_trivial pf_term_ind_trivial pl)
+    | sym p' => sind_sym (pf_sort_ind_trivial p')
+    | trans p1 p2 =>
+      sind_trans (pf_sort_ind_trivial p1) (pf_sort_ind_trivial p2)
+    | conv pt p' =>
+      sind_conv pt p'
+    end.
+
+   Lemma synth_le_args_related' (pl : list pf)  (pa : pf_args_ind pl) c c' el1 el2 args al1 al2
+       : Some (el1,el2) = synth_le_args synth_le_term pl c c' ->
+         Some al1 = get_subseq args (with_names_from c' el1) ->
+         Some al2 = get_subseq args (with_names_from c' el2) ->
+         le_args l c c' (map snd al1) (map snd al2) args el1 el2
+   with synth_le_sort_related' (p : pf)  (ps : pf_sort_ind p) c e1 e2
+    : Some (e1,e2) = synth_le_sort synth_le_term p c ->
+      le_sort l c e1 e2
+   with synth_le_term_related' (p : pf) (pt : pf_term_ind p) c t e1 e2
+    : Some (t,e1,e2) = synth_le_term p c ->
+      le_term l c t e1 e2.
+   Proof.
+     inversion pa;
+        destruct c'; destruct args; break; simpl in *; repeat case_match; intros; simpl in *;
+        repeat (lazymatch goal with
+                | [H : Some _ = Some _|-_] => inversion H; clear H
+                | [H : Some _ = None|-_] => inversion H
+                | [H : None = Some _ |-_] => inversion H
+                | [H : Some _ = named_list_lookup_err _ _ |-_] =>
+                  apply named_list_lookup_err_in in H;
+                  try (let H' := fresh H in
+                       pose proof H as H';
+                       apply rule_in_wf in H'; inversion H'; clear H')
+                | [H : true = (?a == ?b) |-_] =>
+                  symmetry in H;
+                  move: H => /eqP H
+                end; subst; simpl in* ).          
+      { constructor. }
+      {
+        constructor; eauto with imcore.
+        change (le_args l c c' (map (snd (A:=string))  [::]) (map (snd (A:=string)) [::]) [::] l0 l1).
+        eapply synth_le_args_related'; eauto using get_subseq_nil with imcore.
+      }  
+      {
+        revert H5 H6.
+        case seq: (s == s0).
+        {
+          move:seq => /eqP ->.
+          repeat case_match; intros; simpl in *;
+        repeat (lazymatch goal with
+        | [H : Some _ = Some _|-_] => inversion H; clear H
+        | [H : Some _ = None|-_] => inversion H
+        | [H : None = Some _ |-_] => inversion H
+        | [H : Some _ = named_list_lookup_err _ _ |-_] =>
+          apply named_list_lookup_err_in in H;
+            try (let H' := fresh H in
+                 pose proof H as H';
+                 apply rule_in_wf in H'; inversion H'; clear H')
+        | [H : true = (?a == ?b) |-_] =>
+          symmetry in H;
+          move: H => /eqP H
+               end; subst; simpl in* ).
+          constructor; eauto with imcore.
+        }
+        {
+          intros; constructor; eauto with imcore.
+        }
+      }
+      {
+        inversion ps; simpl; repeat case_match; intros;
+        repeat lazymatch goal with
+        | [H : Some _ = Some _|-_] => inversion H; clear H
+        | [H : Some _ = None|-_] => inversion H
+        | [H : None = Some _ |-_] => inversion H
+        | [H : Some _ = named_list_lookup_err _ _ |-_] =>
+          apply named_list_lookup_err_in in H;
+            try (let H' := fresh H in
+                 pose proof H as H';
+                 apply rule_in_wf in H'; inversion H'; clear H')
+        | [H : true = (?a == ?b) |-_] =>
+          symmetry in H;
+          move: H => /eqP H
+               end; subst;
+          eauto with imcore.
+      {
+        eapply le_sort_subst; eauto with imcore.
+        eapply le_subst_from_args.
+        eapply synth_le_args_related'; eauto.
+        eapply get_subseq_exact.
+        assert (map fst (with_names_from c0 l0) = map fst (with_names_from c0 l1)).
+        {
+          rewrite !map_fst_with_names_from; eauto using synth_le_args_size_r, synth_le_args_size_l.
+        }
+        rewrite H0.
+        eapply get_subseq_exact.
+      }
+      }
+      {
+        inversion pt; simpl; repeat case_match; intros;
+        repeat lazymatch goal with
+        | [H : Some _ = Some _|-_] => inversion H; clear H
+        | [H : Some _ = None|-_] => inversion H
+        | [H : None = Some _ |-_] => inversion H
+        | [H : Some _ = named_list_lookup_err _ _ |-_] =>
+          apply named_list_lookup_err_in in H;
+            try (let H' := fresh H in
+                 pose proof H as H';
+                 apply rule_in_wf in H'; inversion H'; clear H')
+        | [H : true = (?a == ?b) |-_] =>
+          symmetry in H;
+          move: H => /eqP H
+               end; subst;
+          eauto with imcore.
+      {
+        eapply le_term_subst; eauto with imcore.
+        eapply le_subst_from_args.
+        eapply synth_le_args_related'; eauto.
+        eapply get_subseq_exact.
+        assert (map fst (with_names_from c0 l0) = map fst (with_names_from c0 l1)).
+        {
+          rewrite !map_fst_with_names_from; eauto using synth_le_args_size_r, synth_le_args_size_l.
+        }
+        rewrite H0.
+        eapply get_subseq_exact.
+      }
+    }
+   Qed.
+
+   Lemma synth_le_args_related (pl : list pf) c c' el1 el2 args al1 al2
+       : Some (el1,el2) = synth_le_args synth_le_term pl c c' ->
+         Some al1 = get_subseq args (with_names_from c' el1) ->
+         Some al2 = get_subseq args (with_names_from c' el2) ->
+         le_args l c c' (map snd al1) (map snd al2) args el1 el2.
+   Proof using wfl.
+     apply synth_le_args_related'; eauto using pf_args_ind_trivial,pf_term_ind_trivial.
+   Qed.
+
+   
+   Lemma synth_le_sort_related (p : pf) c e1 e2
+    : Some (e1,e2) = synth_le_sort synth_le_term p c ->
+      le_sort l c e1 e2.
+   Proof using wfl.
+     apply synth_le_sort_related'; eauto using pf_sort_ind_trivial, pf_args_ind_trivial,pf_term_ind_trivial.
+   Qed.
+
+   Lemma synth_le_term_related (p : pf) c t e1 e2
+    : Some (t,e1,e2) = synth_le_term p c ->
+      le_term l c t e1 e2.
+   Proof using wfl.
+     apply synth_le_term_related'; eauto using pf_term_ind_trivial.
+   Qed.
+   
+
+  Section InnerLoop.
+    Context (synth_wf_term : pf -> ctx -> option (sort*exp)).
+
+    Fixpoint synth_wf_args (pl : list pf) (c c' : ctx) {struct pl}
+      : option (list exp) :=
+      match pl with
+      | [::] => do [::] <- do ret c'; ret ([::])
+      | p::pl' =>
+        do (_,t)::c'' <- do ret c';
+           (t',e) <- synth_wf_term p c;
+           el <- synth_wf_args pl' c c'';
+           ! t' == t[/with_names_from c'' el/];
+           ret (e::el)
+     end.
+  End InnerLoop.
+
+  (* Defined over proof and implicit terms
+   *)
+  Fixpoint synth_wf_term (p : pf) (c : ctx) {struct p} : option (sort*exp) :=
+    match p with
+    | pvar x =>
+      do t <- named_list_lookup_err c x;
+         ret (t,var x)
+    | pcon name pl =>
+      do (term_rule c' args t) <- named_list_lookup_err l name;
+         el <- synth_wf_args synth_wf_term pl c c';
+         al <- get_subseq args (with_names_from c' el);
+         ret (t[/with_names_from c' el/], con name (map snd al))
+    | ax _ _ => None
+    | sym p' => None
+    | trans p1 p2 => None
+    | conv pt p' =>
+      do (t, e) <- synth_wf_term p' c;
+         (t', t1) <- synth_le_sort synth_le_term pt c;
+         ! t == t';
+         ret (t1,e)
+  end.
+
+  Definition synth_wf_sort (pt : pf) (c : ctx) : option sort :=
+      match pt with
+      | pvar x => None
+      | pcon name pl =>
+        do (sort_rule c' args) <- named_list_lookup_err l name;
+           el <- synth_wf_args synth_wf_term pl c c';
+           al <- get_subseq args (with_names_from c' el);
+           ret (scon name (map snd al))
+      | ax _ _ => None
+      | sym p => None
+      | trans p1 p2 => None
+      | conv pt p => None
+  end.
   
 
-Lemma get_subseq_exact (s : subst)
-  : Some s = get_subseq (map fst s) s.
-Proof.
-  induction s; intros; break; simpl in *; auto.
-  rewrite ?eq_refl.
-  rewrite <-IHs; eauto.
-Qed.
+  Fixpoint synth_wf_ctx pl : option ctx :=
+    match pl with
+    | [::] => do ret [::]
+    | (name,p)::pl' =>
+      do c' <- synth_wf_ctx pl';
+         ! fresh name c';
+         t <- synth_wf_sort p c';
+         ret (name,t)::c'
+  end.
+
+   Lemma synth_wf_args_related (pl : list pf) c c' el args al
+       : Some (el) = synth_wf_args synth_wf_term pl c c' ->
+         Some al = get_subseq args (with_names_from c' el) ->
+         wf_args l c (map snd al) args el c'
+   with synth_wf_term_related (p : pf) c t e1 e2
+    : Some (t,e1,e2) = synth_le_term p c ->
+      le_term l c t e1 e2.
+   Proof.
+     {
+       
+       
+End RuleChecking.
+
+Fixpoint refl_pf (e : exp) : pf :=
+  match e with
+  | var x => pvar x
+  | con n l => pcon n (map refl_pf l)
+  end.
+  
+Fixpoint term_step_redex (l : lang) (e : exp) : option (pf*exp) :=
+    match l with
+    | [::] => None
+    | (name,term_le c e1 e2 t)::l' =>
+      (*TODO: check that rule is executable, i.e. FV(e1) >= FV(e2)*)
+      match term_step_redex l' e with
+      | Some t' => Some t'
+      | None => do s <- matches_unordered e e1;
+                ret (ax name (map refl_pf (map snd s)), e2[/s/])
+      end
+    | _::l' => term_step_redex l' e
+    end.
+
+  Fixpoint sort_step_redex (l : lang) (t : sort) : option (pf*sort) :=
+    match l with
+    | [::] => None
+    | (name,sort_le c t1 t2)::l' =>
+      (*TODO: check that rule is executable, i.e. FV(t1) >= FV(t2)*)
+      match sort_step_redex l' t with
+      | Some t' => Some t'
+      | None => do s <- matches_unordered_sort t t1;
+                ret (ax name (map refl_pf (map snd s)),t2[/s/])
+      end
+    | _::l' => sort_step_redex l' t
+    end.
+
+  Section InnerLoop.
+    Context (term_par_step : forall (l : lang) (e : exp), option (pf*exp)).
+    (*TODO: might run afoul of implicits here; probably needs to operate on 
+      full proof terms
+     *)
+    Fixpoint args_par_step l s {struct s} : option (list pf * list exp) :=
+         match s with
+         | [::] => None
+         | e::s' =>
+           match term_par_step l e, args_par_step l s' with
+           | Some e', Some s'' => Some (e'::s'')
+           | Some e', None => Some (e'::s')
+           | None, Some s'' => Some (e::s'')
+           | None, None => None
+           end
+         end.
+  End InnerLoop.
+
+  Fixpoint term_par_step (l : lang) (e : exp) {struct e} : option exp :=
+    match term_step_redex l e, e with
+    | Some e',_ => Some e'
+    | None, var _ => None
+    | None, con name s =>
+      do s' <- args_par_step term_par_step l s;
+      ret (con name s')
+    end.
+  
+  Definition sort_par_step (l : lang) (t:sort) : option sort :=
+    match sort_step_redex l t, t with
+    | Some e',_ => Some e'
+    | None, scon name s =>
+      do s' <- args_par_step term_par_step l s;
+      ret (scon name s')
+    end.
+
+  Fixpoint term_par_step_n (l : lang) (e : exp) (fuel : nat) : exp :=
+    match fuel, term_par_step l e with
+    | 0,_ => e
+    | S _, None => e
+    | S fuel', Some e' => term_par_step_n l e' fuel'
+    end.
+  
+  Fixpoint sort_par_step_n (l : lang) (t : sort) (fuel : nat) : sort :=
+    match fuel, sort_par_step l t with
+    | 0,_ => t
+    | S _, None => t
+    | S fuel', Some t' => sort_par_step_n l t' fuel'
+    end.
+
+
 
